lib/Monads/trace/Trace_No_Fail.thy
@@ -21,7 +21,7 @@ text \<open>
   A monad @{text m} does not fail under precondition @{text P}, if for no start
   state that satisfies the precondition it returns a @{term Failed} result.
 \<close>
-definition no_fail :: "('s \<Rightarrow> bool) \<Rightarrow> ('s,'a) tmonad \<Rightarrow> bool" where
+definition no_fail :: "('c, 's) mpred \<Rightarrow> ('c, 's, 'a) tmonad \<Rightarrow> bool" where
   "no_fail P m \<equiv> \<forall>s. P s \<longrightarrow> \<not> failed (m s)"
 
 
@@ -143,14 +143,14 @@ lemma no_fail_assume_pre:
   "(\<And>s. P s \<Longrightarrow> no_fail P f) \<Longrightarrow> no_fail P f"
   by (simp add: no_fail_def)
 
-\<^cancel>\<open>lemma no_fail_liftM_eq[simp]:
+lemma no_fail_liftM_eq[simp]:
   "no_fail P (liftM f m) = no_fail P m"
-  by (auto simp: liftM_def no_fail_def bind_def return_def)\<close>
+  by (fastforce simp: liftM_def no_fail_def bind_def' return_def failed_def image_def
+               dest!: bspec)
 
 lemma no_fail_liftM[wp]:
   "no_fail P m \<Longrightarrow> no_fail P (liftM f m)"
-  unfolding liftM_def
-  by wpsimp
+  by simp
 
 lemma no_fail_pre_and:
   "no_fail P f \<Longrightarrow> no_fail (P and Q) f"
@@ -162,7 +162,7 @@ lemma no_fail_spec:
 
 lemma no_fail_assertE[wp]:
   "no_fail (\<lambda>_. P) (assertE P)"
-  by (simp add: assertE_def split: if_split)
+  by (simp add: assertE_def)
 
 lemma no_fail_spec_pre:
   "\<lbrakk> no_fail (((=) s) and P') f; \<And>s. P s \<Longrightarrow> P' s \<rbrakk> \<Longrightarrow> no_fail (((=) s) and P) f"
@@ -170,7 +170,7 @@ lemma no_fail_spec_pre:
 
 lemma no_fail_whenE[wp]:
   "\<lbrakk> G \<Longrightarrow> no_fail P f \<rbrakk> \<Longrightarrow> no_fail (\<lambda>s. G \<longrightarrow> P s) (whenE G f)"
-  by (simp add: whenE_def split: if_split)
+  by (simp add: whenE_def)
 
 lemma no_fail_unlessE[wp]:
   "\<lbrakk> \<not> G \<Longrightarrow> no_fail P f \<rbrakk> \<Longrightarrow> no_fail (\<lambda>s. \<not> G \<longrightarrow> P s) (unlessE G f)"
@@ -229,7 +229,7 @@ lemma no_fail_condition[wp]:
 
 lemma no_fail_ex_lift:
   "(\<And>x. no_fail (P x) f) \<Longrightarrow> no_fail (\<lambda>s. \<exists>x. P x s) f"
-  by (fastforce simp: no_fail_def)
+  by (clarsimp simp: no_fail_def)
 
 lemma no_fail_grab_asm:
   "(G \<Longrightarrow> no_fail P f) \<Longrightarrow> no_fail (\<lambda>s. G \<and> P s) f"
