lib/Monads/trace/Trace_Prefix_Closed.thy
@@ -17,7 +17,7 @@ subsection "Prefix Closed"
 text \<open>
   A monad is @{text prefix_closed} if for all traces that it returns, it also returns all incomplete traces
   leading up to it.\<close>
-definition prefix_closed :: "('s, 'a) tmonad \<Rightarrow> bool" where
+definition prefix_closed :: "('c, 's, 'a) tmonad \<Rightarrow> bool" where
   "prefix_closed f = (\<forall>s. \<forall>x xs. (x # xs) \<in> fst ` f s \<longrightarrow> (xs, Incomplete) \<in> f s)"
 
 lemmas prefix_closedD1 = prefix_closed_def[THEN iffD1, rule_format]
