lib/Monads/trace/Trace_In_Monad.thy
@@ -14,32 +14,33 @@ section \<open>Reasoning directly about states\<close>
 (* Lemmas about terms of the form "(v, s') \<in> mres (m s)" *)
 
 lemma in_throwError:
-  "((v, s') \<in> mres (throwError e s)) = (v = Inl e \<and> s' = s)"
+  "((v, s') \<in> mres (throwError e s)) = (v = Inl e \<and> s' = mstate s)"
   by (simp add: throwError_def return_def mres_def)
 
 lemma in_returnOk:
-  "((v', s') \<in> mres (returnOk v s)) = (v' = Inr v \<and> s' = s)"
+  "((v', s') \<in> mres (returnOk v s)) = (v' = Inr v \<and> s' = mstate s)"
   by (simp add: returnOk_def return_def mres_def)
 
 lemma in_bind:
   "((r,s') \<in> mres ((do x \<leftarrow> f; g x od) s)) =
-   (\<exists>s'' x. (x, s'') \<in> mres (f s) \<and> (r, s') \<in> mres (g x s''))"
+   (\<exists>s'' x. (x, s'') \<in> mres (f s) \<and> (r, s') \<in> mres (g x (with_env_of s s'')))"
   by (force simp: bind_def split_def mres_def split: tmres.splits)
 
 lemma in_bindE_R:
   "((Inr r,s') \<in> mres ((doE x \<leftarrow> f; g x odE) s)) =
-  (\<exists>s'' x. (Inr x, s'') \<in> mres (f s) \<and> (Inr r, s') \<in> mres (g x s''))"
+  (\<exists>s'' x. (Inr x, s'') \<in> mres (f s) \<and> (Inr r, s') \<in> mres (g x (with_env_of s s'')))"
   unfolding bindE_def lift_def split_def in_bind
   by (force simp: throwError_def return_def mres_def split: sum.splits)
 
 lemma in_bindE_L:
   "((Inl r, s') \<in> mres ((doE x \<leftarrow> f; g x odE) s)) \<Longrightarrow>
-   (\<exists>s'' x. (Inr x, s'') \<in> mres (f s) \<and> (Inl r, s') \<in> mres (g x s'')) \<or> ((Inl r, s') \<in> mres (f s))"
+   (\<exists>s'' x. (Inr x, s'') \<in> mres (f s) \<and> (Inl r, s') \<in> mres (g x (with_env_of s s'')))
+            \<or> ((Inl r, s') \<in> mres (f s))"
   by (simp add: bindE_def in_bind)
      (force simp: return_def throwError_def lift_def split_def mres_def split: sum.splits if_split_asm)
 
 lemma in_return:
-  "(r, s') \<in> mres (return v s) = (r = v \<and> s' = s)"
+  "(r, s') \<in> mres (return v s) = (r = v \<and> s' = mstate s)"
   by (simp add: return_def mres_def)
 
 lemma in_liftE:
@@ -47,7 +48,7 @@ lemma in_liftE:
   by (force simp: liftE_def in_bind in_return)
 
 lemma in_whenE:
-  "((v, s') \<in> mres (whenE P f s)) = ((P \<longrightarrow> (v, s') \<in> mres (f s)) \<and> (\<not>P \<longrightarrow> v = Inr () \<and> s' = s))"
+  "((v, s') \<in> mres (whenE P f s)) = ((P \<longrightarrow> (v, s') \<in> mres (f s)) \<and> (\<not>P \<longrightarrow> v = Inr () \<and> s' = mstate s))"
   by (simp add: whenE_def in_returnOk)
 
 lemma inl_whenE:
@@ -55,7 +56,7 @@ lemma inl_whenE:
   by (auto simp add: in_whenE)
 
 lemma inr_in_unlessE_throwError[termination_simp]:
-  "(Inr (), s') \<in> mres (unlessE P (throwError E) s) = (P \<and> s'=s)"
+  "(Inr (), s') \<in> mres (unlessE P (throwError E) s) = (P \<and> s' = mstate s)"
   by (simp add: unlessE_def returnOk_def throwError_def in_return)
 
 lemma in_fail:
@@ -63,39 +64,39 @@ lemma in_fail:
   by (simp add: fail_def mres_def)
 
 lemma in_assert:
-  "(r, s') \<in> mres (assert P s) = (P \<and> s' = s)"
+  "(r, s') \<in> mres (assert P s) = (P \<and> s' = mstate s)"
   by (simp add: assert_def return_def fail_def mres_def)
 
 lemma in_assertE:
-  "(r, s') \<in> mres (assertE P s) = (P \<and> r = Inr () \<and> s' = s)"
+  "(r, s') \<in> mres (assertE P s) = (P \<and> r = Inr () \<and> s' = mstate s)"
   by (simp add: assertE_def returnOk_def return_def fail_def mres_def)
 
 lemma in_assert_opt:
-  "(r, s') \<in> mres (assert_opt v s) = (v = Some r \<and> s' = s)"
+  "(r, s') \<in> mres (assert_opt v s) = (v = Some r \<and> s' = mstate s)"
   by (auto simp: assert_opt_def in_fail in_return split: option.splits)
 
 lemma in_get:
-  "(r, s') \<in> mres (get s) = (r = s \<and> s' = s)"
+  "(r, s') \<in> mres (get s) = (r = s \<and> s' = mstate s)"
   by (simp add: get_def mres_def)
 
 lemma in_gets:
-  "(r, s') \<in> mres (gets f s) = (r = f s \<and> s' = s)"
+  "(r, s') \<in> mres (gets f s) = (r = f s \<and> s' = mstate s)"
   by (simp add: simpler_gets_def mres_def)
 
 lemma in_put:
-  "(r, s') \<in> mres (put x s) = (s' = x \<and> r = ())"
+  "(r, s') \<in> mres (put x s) = (s' = mstate x \<and> r = ())"
   by (simp add: put_def mres_def)
 
 lemma in_when:
-  "(v, s') \<in> mres (when P f s) = ((P \<longrightarrow> (v, s') \<in> mres (f s)) \<and> (\<not>P \<longrightarrow> v = () \<and> s' = s))"
+  "(v, s') \<in> mres (when P f s) = ((P \<longrightarrow> (v, s') \<in> mres (f s)) \<and> (\<not>P \<longrightarrow> v = () \<and> s' = mstate s))"
   by (simp add: when_def in_return)
 
 lemma in_unless:
-  "(v, s') \<in> mres (unless P f s) = ((\<not> P \<longrightarrow> (v, s') \<in> mres (f s)) \<and> (P \<longrightarrow> v = () \<and> s' = s))"
+  "(v, s') \<in> mres (unless P f s) = ((\<not> P \<longrightarrow> (v, s') \<in> mres (f s)) \<and> (P \<longrightarrow> v = () \<and> s' = mstate s))"
   by (simp add: unless_def in_when)
 
 lemma in_unlessE:
-  "(v, s') \<in> mres (unlessE P f s) = ((\<not> P \<longrightarrow> (v, s') \<in> mres (f s)) \<and> (P \<longrightarrow> v = Inr () \<and> s' = s))"
+  "(v, s') \<in> mres (unlessE P f s) = ((\<not> P \<longrightarrow> (v, s') \<in> mres (f s)) \<and> (P \<longrightarrow> v = Inr () \<and> s' = mstate s))"
   by (simp add: unlessE_def in_returnOk)
 
 lemma inl_unlessE:
@@ -103,11 +104,11 @@ lemma inl_unlessE:
   by (auto simp add: in_unlessE)
 
 lemma in_modify:
-  "(v, s') \<in> mres (modify f s) = (s'=f s \<and> v = ())"
+  "(v, s') \<in> mres (modify f s) = (s' = mstate (f s) \<and> v = ())"
   by (auto simp add: modify_def bind_def get_def put_def mres_def)
 
 lemma gets_the_in_monad:
-  "((v, s') \<in> mres (gets_the f s)) = (s' = s \<and> f s = Some v)"
+  "((v, s') \<in> mres (gets_the f s)) = (s' = mstate s \<and> f s = Some v)"
   by (auto simp: gets_the_def in_bind in_gets in_assert_opt split: option.split)
 
 lemma in_alternative:
@@ -121,7 +122,7 @@ lemma in_liftM:
 lemma in_bindE:
   "(rv, s') \<in> mres ((f >>=E (\<lambda>rv'. g rv')) s) =
    ((\<exists>ex. rv = Inl ex \<and> (Inl ex, s') \<in> mres (f s)) \<or>
-    (\<exists>rv' s''. (rv, s') \<in> mres (g rv' s'') \<and> (Inr rv', s'') \<in> mres (f s)))"
+    (\<exists>rv' s''. (rv, s') \<in> mres (g rv' (with_env_of s s'')) \<and> (Inr rv', s'') \<in> mres (f s)))"
   apply (clarsimp simp: bindE_def in_bind lift_def in_throwError)
   apply (safe del: disjCI; strengthen subst[where P="\<lambda>x. x \<in> mres (f s)", mk_strg I _ E];
          auto simp: in_throwError split: sum.splits)
@@ -135,19 +136,19 @@ lemmas in_monad = inl_whenE in_whenE in_liftE in_bind in_bindE_L
                   in_alternative in_liftM
 
 lemma bind_det_exec:
-  "mres (a s) = {(r,s')} \<Longrightarrow> mres ((a >>= b) s) = mres (b r s')"
+  "mres (a s) = {(r,s')} \<Longrightarrow> mres ((a >>= b) s) = mres (b r (with_env_of s s'))"
   by (simp add: in_bind set_eq_iff)
 
 lemma in_bind_det_exec:
-  "mres (a s) = {(r,s')} \<Longrightarrow> (s'' \<in> mres ((a >>= b) s)) = (s'' \<in> mres (b r s'))"
+  "mres (a s) = {(r,s')} \<Longrightarrow> (s'' \<in> mres ((a >>= b) s)) = (s'' \<in> mres (b r (with_env_of s s')))"
   by (cases s'', simp add: in_bind)
 
 lemma exec_put:
-  "(put s' >>= m) s = m () s'"
+  "(put s' >>= m) s = m () (with_env_of s (mstate s'))"
   by (simp add: bind_def put_def mres_def split_def)
 
 lemma bind_execI:
-  "\<lbrakk> (r'',s'') \<in> mres (f s); \<exists>x \<in> mres (g r'' s''). P x \<rbrakk> \<Longrightarrow> \<exists>x \<in> mres ((f >>= g) s). P x"
+  "\<lbrakk> (r'',s'') \<in> mres (f s); \<exists>x \<in> mres (g r'' (with_env_of s s'')). P x \<rbrakk> \<Longrightarrow> \<exists>x \<in> mres ((f >>= g) s). P x"
   by (force simp: Bex_def in_bind)
 
 end
