lib/Monads/trace/Trace_Reader_Option.thy
@@ -23,7 +23,7 @@ translations
   "_doO (_nobind b) e"     == "b |>> (CONST K_bind e)"
   "DO x <- a; e OD"        == "a |>> (\<lambda>x. e)"
 
-
+(* These are here, because K_bind is not available yet in Reader_Option_VCG *)
 lemma ovalid_K_bind_wp[wp]:
   "ovalid P f Q \<Longrightarrow> ovalid P (K_bind f x) Q"
   by simp
@@ -36,8 +36,15 @@ lemma no_ofail_K_bind[wp]:
   "no_ofail P f \<Longrightarrow> no_ofail P (K_bind f x)"
   by simp
 
+(* The connection between the reader option monad and the trace monad is the trace operator
+   "gets_the". We generally want the environment state of the trace monad to be available to
+   the reader option monad, since the reader monad may want to make decisions that depend on
+   the environment state. Because gets_the is constructed via gets, it has the whole monad
+   state available, including the environment part. This makes it possible to use the same P
+   in the following rule for the reader option monad and the trace monad, without any type
+   lifting. *)
 lemma no_ofail_gets_the_eq:
-  "no_ofail P f \<longleftrightarrow> no_fail P (gets_the (f :: ('s, 'a) lookup))"
+  "no_ofail P f \<longleftrightarrow> no_fail P (gets_the f)"
   by (auto simp: no_ofail_def no_fail_def gets_the_def gets_def
                  get_def assert_opt_def bind_def return_def fail_def
          split: option.split)
@@ -46,7 +53,10 @@ lemmas no_ofail_gets_the =
   no_ofail_gets_the_eq[THEN iffD1]
 
 
-(* Lemmas relating ovalid and valid *)
+(* Lemmas relating ovalid and valid. See comment above for no_ofail_gets_the_eq -- we can use
+   P and Q with the same type here, because of our choice of type for get/gets/get_the.
+   Similarly, the gets_the f rewrites below are possible to write nicely because the types
+   coincide. *)
 lemma ovalid_gets_the:
   "ovalid P f Q \<Longrightarrow> \<lbrace>P\<rbrace> gets_the f \<lbrace>Q\<rbrace>"
   apply wpsimp
@@ -104,7 +114,7 @@ lemma gets_the_assert:
 
 lemma gets_the_ostate_assert:
   "gets_the (ostate_assert P) = state_assert P"
-  by (clarsimp simp: ostate_assert_def state_assert_def gets_the_obind gets_the_Some_get
+  by (clarsimp simp: ostate_assert_def state_assert_def gets_the_Some_get gets_the_obind
                      gets_the_assert)
 
 lemma gets_the_assert_opt:
@@ -129,7 +139,7 @@ lemma gets_obind_bind_eq:
   by (auto simp: simpler_gets_def bind_def obind_def return_def split: option.splits)
 
 lemma mres_assert_opt:
-  "mres (assert_opt opt s) = (if opt = None then {} else {(the opt,s)})"
+  "mres (assert_opt opt s) = (if opt = None then {} else {(the opt, mstate s)})"
   by (clarsimp simp: assert_opt_def fail_def return_def mres_def vimage_def split: option.split)
 
 
@@ -145,23 +155,24 @@ section "Relation between option monad loops and trace monad loops."
 (* Option monad whileLoop formalisation thanks to Lars Noschinski <noschinl@in.tum.de>. *)
 
 lemma gets_the_conv:
-  "(gets_the B s) = (case B s of Some r' \<Rightarrow> ({([], Result (r', s))}) | _ \<Rightarrow> {([], Failed)})"
-  by (auto simp: gets_the_def gets_def get_def bind_def return_def fail_def assert_opt_def split: option.splits)
+  "(gets_the B s) = (case B s of Some r' \<Rightarrow> ({([], Result (r', mstate s))}) | _ \<Rightarrow> {([], Failed)})"
+  by (auto simp: gets_the_def gets_def get_def bind_def return_def fail_def assert_opt_def
+           split: option.splits)
 
 lemma gets_the_loop_terminates:
-  "whileLoop_terminates C (\<lambda>a. gets_the (B a)) r s
-    \<longleftrightarrow> (\<exists>rs'. (Some r, rs') \<in> option_while' (\<lambda>a. C a s) (\<lambda>a. B a s))" (is "?L \<longleftrightarrow> ?R")
+  "whileLoop_terminates C (\<lambda>a. gets_the (B a)) c r s
+    \<longleftrightarrow> (\<exists>rs'. (Some r, rs') \<in> option_while' (\<lambda>a. C a (monad_state c s)) (\<lambda>a. B a (monad_state c s)))" (is "?L \<longleftrightarrow> ?R")
 proof
   assume ?L then show ?R
   proof (induct rule: whileLoop_terminates.induct[case_names 1 2])
     case (2 r s) then show ?case
-      by (cases "B r s") (auto simp: gets_the_conv intro: option_while'.intros)
+      by (cases "B r (monad_state c s)") (auto simp: gets_the_conv intro: option_while'.intros)
   qed (auto intro: option_while'.intros)
 next
   assume ?R then show ?L
   proof (elim exE)
-    fix rs' assume "(Some r, rs') \<in> option_while' (\<lambda>a. C a s) (\<lambda>a. B a s)"
-    then have "whileLoop_terminates C (\<lambda>a. gets_the (B a)) (the (Some r)) s"
+    fix rs' assume "(Some r, rs') \<in> option_while' (\<lambda>a. C a (monad_state c s)) (\<lambda>a. B a (monad_state c s))"
+    then have "whileLoop_terminates C (\<lambda>a. gets_the (B a)) c (the (Some r)) s"
       by induct (auto intro: whileLoop_terminates.intros simp: gets_the_conv)
     then show ?thesis by simp
   qed
@@ -172,54 +183,76 @@ lemma The_eqD:
   by (metis theI)
 
 lemma gets_the_whileLoop:
-  fixes C :: "'a \<Rightarrow> 's \<Rightarrow> bool"
-  assumes terminates: "\<forall>s. whileLoop_terminates C (\<lambda>a. gets_the (B a)) r s"
+  fixes C :: "'a \<Rightarrow> ('c, 's) monad_state \<Rightarrow> bool"
+  assumes terminates: "\<forall>s. whileLoop_terminates C (\<lambda>a. gets_the (B a)) (env s) r (mstate s)"
   shows "whileLoop C (\<lambda>a. gets_the (B a)) r = gets_the (owhile C B r)"
 proof -
-  { fix r s r' s' ts assume "((r,s), ts, Result (r', s')) \<in> whileLoop_results C (\<lambda>a. gets_the (B a))"
-    then have "s = s' \<and> ts = [] \<and>(Some r, Some r') \<in> option_while' (\<lambda>a. C a s) (\<lambda>a. B a s)"
+  {
+    fix r s r' s' c ts
+    assume "((r,s), ts, Result (r', s')) \<in> whileLoop_results C (\<lambda>a. gets_the (B a)) c"
+    then
+    have "s = s' \<and> ts = [] \<and>
+          (Some r, Some r') \<in> option_while' (\<lambda>a. C a (monad_state c s)) (\<lambda>a. B a (monad_state c s))"
     by (induct r s ts "Result (r', s')")
-       (auto intro: option_while'.intros simp: gets_the_conv split: option.splits) }
+       (auto intro: option_while'.intros simp: gets_the_conv split: option.splits)
+  }
   note wl'_Result = this
 
-  { fix r s ts assume "((r,s), ts, Failed) \<in> whileLoop_results C (\<lambda>a. gets_the (B a))"
-    then have "ts = [] \<and> (Some r, None) \<in> option_while' (\<lambda>a. C a s) (\<lambda>a. B a s)"
+  {
+    fix r s c ts
+    assume "((r,s), ts, Failed) \<in> whileLoop_results C (\<lambda>a. gets_the (B a)) c"
+    then
+    have "ts = [] \<and>
+          (Some r, None) \<in> option_while' (\<lambda>a. C a (monad_state c s)) (\<lambda>a. B a (monad_state c s))"
       by (induct r s ts "Failed :: (('s, 'a) tmres)")
-         (auto intro: option_while'.intros simp: gets_the_conv split: option.splits) }
+         (auto intro: option_while'.intros simp: gets_the_conv split: option.splits)
+  }
   note wl'_Failed = this
 
-  { fix r s ts assume "((r,s), ts, Incomplete) \<in> whileLoop_results C (\<lambda>a. gets_the (B a))"
-    then have "False"
+  {
+    fix r s c ts
+    assume "((r,s), ts, Incomplete) \<in> whileLoop_results C (\<lambda>a. gets_the (B a)) c"
+    then
+    have "False"
       by (induct r s ts "Incomplete :: (('s, 'a) tmres)")
-         (auto intro: option_while'.intros simp: gets_the_conv split: option.splits) }
+         (auto intro: option_while'.intros simp: gets_the_conv split: option.splits)
+  }
   note wl'_Incomplete = this
 
-  { fix r s r' assume "(Some r, Some r') \<in> option_while' (\<lambda>a. C a s) (\<lambda>a. B a s)"
-    then have "((r,s), [], Result (r',s)) \<in> whileLoop_results C (\<lambda>a. gets_the (B a))"
+  {
+    fix r s r' c
+    assume "(Some r, Some r') \<in> option_while' (\<lambda>a. C a (monad_state c s)) (\<lambda>a. B a (monad_state c s))"
+    then
+    have "((r,s), [], Result (r',s)) \<in> whileLoop_results C (\<lambda>a. gets_the (B a)) c"
     by (induct "Some r" "Some r'" arbitrary: r)
-       (auto intro: whileLoop_results.intros simp: gets_the_conv) }
+       (auto intro: whileLoop_results.intros simp: gets_the_conv)
+  }
   note option_while'_Some = this
 
-  { fix r s assume "(Some r, None) \<in> option_while' (\<lambda>a. C a s) (\<lambda>a. B a s)"
-    then have "((r,s), [], Failed) \<in> whileLoop_results C (\<lambda>a. gets_the (B a))"
+  {
+    fix r s c
+    assume "(Some r, None) \<in> option_while' (\<lambda>a. C a (monad_state c s)) (\<lambda>a. B a (monad_state c s))"
+    then have "((r,s), [], Failed) \<in> whileLoop_results C (\<lambda>a. gets_the (B a)) c"
     by (induct "Some r" "None :: 'a option" arbitrary: r)
-       (auto intro: whileLoop_results.intros simp: gets_the_conv) }
+       (auto intro: whileLoop_results.intros simp: gets_the_conv)
+  }
   note option_while'_None = this
 
-  have "\<And>s. owhile C B r s = None
-          \<Longrightarrow> whileLoop C (\<lambda>a. gets_the (B a)) r s = {([], Failed)}"
+  have "\<And>s. owhile C B r s = None \<Longrightarrow> whileLoop C (\<lambda>a. gets_the (B a)) r s = {([], Failed)}"
     using terminates
+    unfolding whileLoop_def owhile_def option_while_def
     by (intro subset_antisym;
-        clarsimp simp: whileLoop_def owhile_def option_while_def gets_the_loop_terminates
+        clarsimp simp: gets_the_loop_terminates
                 split: if_split_asm intro!: option_while'_None dest!: The_eqD)
        (case_tac b, auto dest!: wl'_Result wl'_Failed wl'_Incomplete option_while'_inj option_while'_THE)
   moreover
   have "\<And>s r'. owhile C B r s = Some r'
-          \<Longrightarrow> whileLoop C (\<lambda>a. gets_the (B a)) r s = {([], Result (r', s))}"
+                \<Longrightarrow> whileLoop C (\<lambda>a. gets_the (B a)) r s = {([], Result (r', mstate s))}"
+    unfolding whileLoop_def owhile_def option_while_def
     by (intro subset_antisym;
-        clarsimp simp: whileLoop_def owhile_def option_while_def option_while'_THE
+        clarsimp simp: option_while'_THE
                 split: if_split_asm intro!: option_while'_Some)
-       (case_tac b, auto dest: wl'_Result wl'_Failed wl'_Incomplete option_while'_inj)
+       (case_tac b, auto dest!: wl'_Result wl'_Failed wl'_Incomplete dest: option_while'_inj)
   ultimately
   show ?thesis
     by (auto simp: fun_eq_iff gets_the_conv split: option.split)
